```
// 01 → w
z = w + 1

// 02 → w
z *= 26
z += w + 9

// 03 → w
z *= 26
z += w + 11

// 04 → w
x = (z % 26 - 13) != w
z /= 26
z *= 25 * x + 1
z += (w + 6) * x

// 05 → w
z *= 26
z += w + 6

// 06 → w
z *= 26
z += w + 13

// 07 → w
x = (z % 26 - 14) != w
z /= 26
z *= 25 * x + 1
z += (w + 13) * x

// 08 → w
z *= 26
z += w + 5

// 09 → w
x = (z % 26 - 8) != w
z /= 26
z *= 25 * x + 1
z += (w + 7) * x

// 10 → w
z *= 26
z += w + 2

// 11 → w
x = (z % 26 - 9) != w
z /= 26
z *= 25 * x + 1
z += (w + 10) * x

// 12 → w
x = (z % 26 - 11) != w
z /= 26
z *= 25 * x + 1
z += (w + 14) * x

// 13 → w
x = (z % 26 - 6) != w
z /= 26
z *= 25 * x + 1
z += (w + 7) * x

// 14 → w
x = (z % 26 - 5) != w
z /= 26
z *= 25 * x + 1
z += (w + 1) * x
```
